working way through 23trees...

src/Data/Ext.v
@@ -1,150 +1,151 @@
 Require Import FP.Structures.EqDec.
 Require Import FP.Structures.Eqv.
 Require Import FP.Structures.Lattice.
+Require Import FP.Structures.Additive.
 Require Import FP.Structures.Injection.
+Require Import FP.Structures.Deriving.
 Require Import FP.Data.Option.
 Require Import FP.Structures.Ord.
 Require Import FP.Data.Function.
 Require Import FP.Data.Sum.
 Require Import FP.Data.Unit.
+Require Import FP.Relations.Setoid.
 
+Import AdditiveNotation.
 Import FunctionNotation.
 Import LatticeNotation.
 Import OrdNotation.
 
 Definition ext_bot := option.
 
-Section ext_top.
-  Inductive ext_top A := ExtTop { un_ext_top : option A }.
-  Global Arguments ExtTop {A} _.
-  Global Arguments un_ext_top {A} _.
+Inductive ext_top A := ExtTop { un_ext_top : option A }.
+Global Arguments ExtTop {A} _.
+Global Arguments un_ext_top {A} _.
 
-  Definition ext_top_to_sum {A} (et:ext_top A) : A + unit :=
+Section ext_top_Bijection.
+  Context {A:Type}.
+
+  Definition ext_top_to_sum (et:ext_top A) : A + unit :=
     match un_ext_top et with
     | None => inr tt
     | Some a => inl a
     end.
+  Global Instance ext_top_sum_InjectionRespect_eq
+      : InjectionRespect (ext_top A) (A+unit) ext_top_to_sum eq eq.
+  Proof. constructor ; unfold Proper ; simpl in * ; intros.
+    congruence.
+    destruct x as [x], y as [y] ; destruct x,y ; simpl in * ;
+      unfold ext_top_to_sum in H ; simpl in H ; try congruence.
+  Qed.
 
-  Section EqDec.
-    Context {A} {E:EqDec A}.
+  Definition sum_to_ext_top (et:A+unit) : ext_top A :=
+    ExtTop $
+      match et with
+      | inr tt => None
+      | inl a => Some a
+      end.
+  Global Instance sum_ext_top_InjectionInverse_eq
+      : InjectionInverse (A+unit) (ext_top A) sum_to_ext_top ext_top_to_sum eq.
+  Proof. constructor ; intros ;
+      destruct x ; [ idtac | destruct u ] ; simpl ; unfold ext_top_to_sum ; simpl ;
+      auto.
+  Qed.
+End ext_top_Bijection.
 
-    Global Instance ext_top_EqDec : EqDec (ext_top A) :=
-      { eq_dec := eq_dec `on` ext_top_to_sum }.
-  End EqDec.
+Module ext_top_DTKS1_Arg <: DerivingTheKitchenSink1_Arg.
+  Definition T A := ext_top A.
+  Definition U A := A+(unit:Type).
+  Definition to {A} (x:T A) := ext_top_to_sum x.
+  Definition from {A} (x:U A) := sum_to_ext_top x.
+  Definition InjResp A : InjectionRespect (T A) (U A) to eq eq := _.
+  Definition InjInv A : InjectionInverse (U A) (T A) from to eq := _.
+End ext_top_DTKS1_Arg.
 
-  Section Eqv.
-    Context {A} {E:Eqv A}.
+Module ext_top_DTKS1 := DerivingTheKitchenSink1 ext_top_DTKS1_Arg.
+Import ext_top_DTKS1.
 
-    Global Instance ext_top_Eqv : Eqv (ext_top A) :=
-      { eqv := eqv `on` ext_top_to_sum }.
-  End Eqv.
+Inductive ext_top_bot A := ExtTopBot { un_ext_top_bot : option (option A) }.
+Global Arguments ExtTopBot {A} _.
+Global Arguments un_ext_top_bot {A} _.
 
-  Section EqvDec.
-    Context {A} {E:EqvDec A}.
+Section ext_top_bot_Bijection.
+  Context {A:Type}.
 
-    Global Instance ext_top_EqvDec : EqvDec (ext_top A) :=
-      { eqv_dec := eqv_dec `on` ext_top_to_sum }.
-  End EqvDec.
-
-  Section Ord.
-    Context {A} {E:Ord A}.
-
-    Global Instance ext_top_Ord : Ord (ext_top A) :=
-      { lt := lt `on` ext_top_to_sum }.
-  End Ord.
-
-  Section OrdDec.
-    Context {A} {O:OrdDec A}.
-
-    Global Instance ext_top_OrdDec : OrdDec (ext_top A) :=
-      { ord_dec := ord_dec `on` ext_top_to_sum }.
-  End OrdDec.
-End ext_top.
-
-Section ext_top_bot.
-  Inductive ext_top_bot A := ExtTopBot { un_ext_top_bot : option (option A) }.
-  Global Arguments ExtTopBot {A} _.
-  Global Arguments un_ext_top_bot {A} _.
-
-  Global Instance ext_top_bot_Injection {A} : HasInjection A (ext_top_bot A) :=
-    { inject := ExtTopBot '.' Some '.' Some }.
-
-  Definition ext_top_bot_to_sum {A} (e:ext_top_bot A) : unit + A + unit :=
+  Definition ext_top_bot_to_sum (e:ext_top_bot A) : unit + A + unit :=
     match un_ext_top_bot e with
     | None => inr tt
     | Some None => inl (inl tt)
     | Some (Some a) => inl (inr a)
     end.
+  Global Instance ext_top_bot_InjectionRespect_eq
+      : InjectionRespect (ext_top_bot A) (unit+A+unit) ext_top_bot_to_sum eq eq.
+  Proof. constructor ; unfold Proper ; simpl ; intros.
+    congruence.
+    unfold ext_top_bot_to_sum in H.
+    destruct x as [x], y as [y] ;
+      destruct x as [ x |], y as [y |] ;
+      [ destruct x,y | destruct x | destruct y |] ;
+      simpl in * ; congruence.
+  Qed.
 
-  Section EqDec.
-    Context {A} {E:EqDec A}.
-
-    Global Instance ext_top_bot_EqDec : EqDec (ext_top_bot A) :=
-      { eq_dec := eq_dec `on` ext_top_bot_to_sum }.
-  End EqDec.
-
-  Section Eqv.
-    Context {A} {E:Eqv A}.
-
-    Global Instance ext_top_bot_Eqv : Eqv (ext_top_bot A) :=
-      { eqv := eqv `on` ext_top_bot_to_sum }.
-  End Eqv.
-
-  Section EqvDec.
-    Context {A} {E:EqvDec A}.
-
-    Global Instance ext_top_bot_EqvDec : EqvDec (ext_top_bot A) :=
-      { eqv_dec := eqv_dec `on` ext_top_bot_to_sum }.
-  End EqvDec.
-
-  Section Ord.
-    Context {A} {E:Ord A}.
-
-    Global Instance ext_top_bot_Ord : Ord (ext_top_bot A) :=
-      { lt := lt `on` ext_top_bot_to_sum }.
-  End Ord.
-
-  Section OrdDec.
-    Context {A} {O:OrdDec A}.
-
-    Global Instance ext_top_bot_OrdDec : OrdDec (ext_top_bot A) :=
-      { ord_dec := ord_dec `on` ext_top_bot_to_sum }.
-  End OrdDec.
-
-  Section Lattice.
-    Context {A} {E:Eqv A} {EWF:EqvWF A} {O:Ord A} {OWF:OrdWF A} {L:Lattice A} {LWF:LatticeWF A}.
-
-    Definition ext_top_bot_meet (e1:ext_top_bot A) (e2:ext_top_bot A)
-        : ext_top_bot A := ExtTopBot $
-      match un_ext_top_bot e1, un_ext_top_bot e2 with
-      | None, e2 => e2
-      | e1, None => e1
-      | Some None, _ => Some None
-      | _, Some None => Some None
-      | Some (Some a1), Some (Some a2) => Some $ Some (a1 /\ a2)
+  Definition sum_to_ext_top_bot (e:unit+A+unit) : ext_top_bot A :=
+    ExtTopBot $
+      match e with
+      | inr tt => None
+      | inl (inl tt) => Some None
+      | inl (inr a) => Some (Some a)
       end.
+  Global Instance sum_ext_top_bot_InjectionInverse_eq
+      : InjectionInverse (unit+A+unit) (ext_top_bot A)
+                         sum_to_ext_top_bot ext_top_bot_to_sum eq.
+  Proof. constructor ; intros.
+    destruct x as [x | u] ; [destruct x as [u | x] ; [destruct u |] | destruct u] ;
+      unfold ext_top_bot_to_sum ; simpl in * ; congruence.
+  Qed.
+End ext_top_bot_Bijection.
 
-    Definition ext_top_bot_join (e1:ext_top_bot A) (e2:ext_top_bot A)
-        : ext_top_bot A := ExtTopBot $
-      match un_ext_top_bot e1, un_ext_top_bot e2 with
-      | None, _ => None
-      | _, None => None
-      | Some None, e2 => e2
-      | e1, Some None => e1
-      | Some (Some a1), Some (Some a2) => Some $ Some (a1 \/ a2)
-      end.
+Module ext_top_bot_DTKS1_Arg <: DerivingTheKitchenSink1_Arg.
+  Definition T A := ext_top_bot A.
+  Definition U A := (unit:Type)+A+unit.
+  Definition to {A} (x:T A) := ext_top_bot_to_sum x.
+  Definition from {A} (x:U A) := sum_to_ext_top_bot x.
+  Definition InjResp A : InjectionRespect (T A) (U A) to eq eq := _.
+  Definition InjInv A : InjectionInverse (U A) (T A) from to eq := _.
+End ext_top_bot_DTKS1_Arg.
 
-    Definition ext_top_bot_top : ext_top_bot A := ExtTopBot None.
-    Definition ext_top_bot_bot : ext_top_bot A := ExtTopBot $ Some None.
+Module ext_top_bot_DTKS1 := DerivingTheKitchenSink1 ext_top_bot_DTKS1_Arg.
+Import ext_top_bot_DTKS1.
 
-    Global Instance ext_top_bot_Lattice : Lattice (ext_top_bot A) :=
-      { lmeet := ext_top_bot_meet
-      ; ljoin := ext_top_bot_join
-      }.
-    Global Instance ext_top_bot_BoundedLattice : BoundedLattice (ext_top_bot A) :=
-      { ltop := ext_top_bot_top
-      ; lbot := ext_top_bot_bot
-      }.
+Section Injection.
+  Context {A:Type} {E:Eqv A}.
 
-  End Lattice.
-End ext_top_bot.
+  Global Instance ext_top_bot_HasInjection : HasInjection A (ext_top_bot A) :=
+    { inject := ExtTopBot '.' Some '.' Some }.
+  Global Instance ext_top_bot_InjectionRespect_inject_eq
+      : InjectionRespect A (ext_top_bot A) inject eq eq.
+  Proof. constructor ; unfold Proper ; simpl ; intros.
+    congruence.
+    unfold inject in H ; simpl in H ; congruence.
+  Qed.
+  Global Instance ext_top_bot_InjectionRespect_inject_eqv
+      : InjectionRespect A (ext_top_bot A) inject eqv eqv.
+  Proof. constructor ; unfold Proper ; simpl ; intros.
+    unfold eqv, inject ; simpl ; unfold ext_top_bot_to_sum ; simpl.
+    rewrite <- H.
+    (* here. set up injection respect relations for sum and option then here.  try to generalize.  then proceed with 23trees. *)
+    DerivingInjResp inject eqv eqv _.
+  Proof. unfold eqv ; simpl.
+
+  Context {A_Ord:Ord A} {A_BoundedLattice:BoundedLattice A}.
+
+  Lemma ext_top_bot_inject_ineq :
+    forall (a:A), lbot < (inject (U:=ext_top_bot A)) a < ltop.
+  Proof. intros ; constructor.
+    apply InjectionRespect_beta ; simpl.
+      compute.
+      repeat constructor.
+    apply InjectionRespect_beta ; simpl.
+      compute.
+      repeat constructor.
+  Qed.
+End Injection.
