src/Data/TwoThreeTreesWF.v
@@ -1,6 +1,8 @@
 Require Import FP.Data.TwoThreeTrees.
 Require Import FP.Structures.WellFormed.
 Require Import FP.Data.N.
+Require Import FP.Data.Unit.
+Require Import FP.Data.Sum.
 Require Import FP.Data.Ext.
 Require Import FP.Structures.Peano.
 Require Import FP.Structures.Lattice.
@@ -8,75 +10,302 @@ Require Import FP.Structures.Injection.
 Require Import FP.Structures.Ord.
 Require Import FP.Structures.Eqv.
 Require Import FP.Structures.Additive.
+Require Import FP.Relations.RelDec.
 
 Import OrdNotation.
 Import AdditiveNotation.
 
-
 Module TwoThreeTreesWF.
   Import TwoThreeTrees.
 
-  Inductive tree_iwf {K V} {Lat:Lattice K} {O:Ord K}
-      : ext_top_bot K -> ext_top_bot K -> N -> tree K V -> Prop :=
-    | NullWF : forall t_lower_bound t_upper_bound,
-                 tree_iwf t_lower_bound t_upper_bound 0 Null_t
-    | TwoWF : forall tl_lower_bound tl_upper_bound
-                     tr_lower_bound tr_upper_bound
-                     t_height
-                     tl km vm tr,
-                tree_iwf tl_lower_bound tl_upper_bound t_height tl
-             -> tree_iwf tr_lower_bound tr_upper_bound t_height tr
-             -> tl_upper_bound < inject km < tr_lower_bound
-             -> tree_iwf tl_lower_bound tr_upper_bound
-                         (t_height+1)
-                         (Two_t tl (km,vm) tr)
-    | ThreeWF : forall tl_lower_bound tl_upper_bound
-                       tm_lower_bound tm_upper_bound
-                       tr_lower_bound tr_upper_bound
-                       t_height
-                       tl kl vl tm kr vr tr,
-                  tree_iwf tl_lower_bound tl_upper_bound t_height tl
-               -> tree_iwf tm_lower_bound tm_upper_bound t_height tm
-               -> tree_iwf tr_lower_bound tr_upper_bound t_height tr
-               -> tl_upper_bound < inject kl < tm_lower_bound
-               -> tm_upper_bound < inject kr < tr_lower_bound
-               -> tree_iwf tl_lower_bound tr_upper_bound
-                           (t_height+1)
-                           (Three_t tl (kl,vl) tm (kr,vr) tr).
-
-  Definition tree_wf {K V} {Lat:Lattice K} {O:Ord K} (t:tree K V) : Prop :=
-    exists n:N, tree_iwf lbot ltop n t.
-
-  Global Instance tree_WellFormed {K V} {Lat:Lattice K} {O:Ord K}
-    : WellFormed (tree K V) := { wf := tree_wf }.
-
-  Section wf.
-    Context {K} {KE:Eqv K} {KOrd:OrdDec K} {KO:Ord K} {KLat:Lattice K} {LWF:LatticeWF K}.
+  Section Context.
+    Context {K:Type}.
+    Context {E:Eqv K}.
+    Context {O:Ord K} {OWF:OrdWF K}.
+    Context {L:Lattice K} {B:BoundedLattice K}.
+    Context {OD:OrdDec K} {ODC:OrdDecCorrect K}.
     Context {V:Type}.
 
-    Definition empty_wf : with_wf (tree K V).
-      refine(
-        ex_intro _ empty _
-      ).
-      simpl.
-      exists 0.
-      econstructor.
-    Defined.
+    Inductive tree_iwf : ext_top_bot K -> ext_top_bot K -> N -> tree K V -> Prop :=
+      | NullWF :
+          forall
+            t_lower_bound t_upper_bound,
+              tree_iwf t_lower_bound t_upper_bound 0 Null_t
+      | TwoWF :
+          forall
+            tl tl_lower_bound tl_upper_bound
+            tr tr_lower_bound tr_upper_bound
+            t_height
+            km vm,
+              tree_iwf tl_lower_bound tl_upper_bound t_height tl
+           -> tree_iwf tr_lower_bound tr_upper_bound t_height tr
+           -> tl_upper_bound < inject km < tr_lower_bound
+           -> tree_iwf tl_lower_bound tr_upper_bound (t_height+1)
+                       (Two_t tl (km,vm) tr)
+      | ThreeWF :
+          forall
+            tl tl_lower_bound tl_upper_bound
+            tm tm_lower_bound tm_upper_bound
+            tr tr_lower_bound tr_upper_bound
+            t_height
+            kl vl kr vr,
+              tree_iwf tl_lower_bound tl_upper_bound t_height tl
+           -> tree_iwf tm_lower_bound tm_upper_bound t_height tm
+           -> tree_iwf tr_lower_bound tr_upper_bound t_height tr
+           -> tl_upper_bound < inject kl < tm_lower_bound
+           -> tm_upper_bound < inject kr < tr_lower_bound
+           -> tree_iwf tl_lower_bound tr_upper_bound (t_height+1)
+                       (Three_t tl (kl,vl) tm (kr,vr) tr).
 
-    Definition singleton_wf (k:K) (v:V) : with_wf (tree K V).
-      refine(
-        ex_intro _ (singleton k v) _
-      ).
-      simpl.
-      exists (0+1).
-      eapply (TwoWF _ lbot ltop _).
-      econstructor.
-      econstructor.
-      eauto.
+    Inductive context_iwf
+        : ext_top_bot K -> ext_top_bot K -> N (* bounds and height of hole *)
+       -> ext_top_bot K -> ext_top_bot K -> N (* bounds and height when filled *)
+       -> context K V
+       -> Prop :=
+      | TopWF :
+          forall
+            t_lower_bound t_upper_bound
+            t_height,
+              context_iwf t_lower_bound t_upper_bound t_height
+                          t_lower_bound t_upper_bound t_height Top_c
+      | TwoLeftHoleWF :
+          forall
+            h_lower_bound h_upper_bound h_height
+            tr tr_lower_bound tr_upper_bound
+            c c_lower_bound c_upper_bound c_height
+            k v,
+              context_iwf h_lower_bound tr_upper_bound (h_height+1)
+                          c_lower_bound c_upper_bound c_height c
+           -> tree_iwf tr_lower_bound tr_upper_bound h_height tr
+           -> h_upper_bound < inject k < tr_lower_bound
+           -> context_iwf h_lower_bound h_upper_bound h_height
+                          c_lower_bound c_upper_bound c_height
+                          (TwoLeftHole_c (k,v) tr c)
+      | TwoRightHoleWF :
+          forall
+            h_lower_bound h_upper_bound h_height
+            tl tl_lower_bound tl_upper_bound
+            c c_lower_bound c_upper_bound c_height
+            k v,
+              context_iwf tl_lower_bound h_upper_bound (h_height+1)
+                          c_lower_bound c_upper_bound c_height c
+           -> tree_iwf tl_lower_bound tl_upper_bound h_height tl
+           -> tl_upper_bound < inject k < h_lower_bound
+           -> context_iwf h_lower_bound h_upper_bound h_height
+                          c_lower_bound c_upper_bound c_height
+                          (TwoRightHole_c tl (k,v) c)
+      | ThreeLeftHoleWF :
+          forall
+            h_lower_bound h_upper_bound h_height
+            tm tm_lower_bound tm_upper_bound
+            tr tr_lower_bound tr_upper_bound
+            c c_lower_bound c_upper_bound c_height
+            kl vl kr vr,
+              context_iwf h_lower_bound tr_upper_bound (h_height+1)
+                          c_lower_bound c_upper_bound c_height c
+           -> tree_iwf tm_lower_bound tm_upper_bound h_height tm
+           -> tree_iwf tr_lower_bound tr_upper_bound h_height tr
+           -> h_upper_bound < inject kl < tm_lower_bound
+           -> tm_upper_bound < inject kr < tr_lower_bound
+           -> context_iwf h_lower_bound h_upper_bound h_height
+                          c_lower_bound c_upper_bound c_height
+                          (ThreeLeftHole_c (kl,vl) tm (kr,vr) tr c)
+      | ThreeMiddleHoleWF :
+          forall
+            h_lower_bound h_upper_bound h_height
+            tl tl_lower_bound tl_upper_bound
+            tr tr_lower_bound tr_upper_bound
+            c c_lower_bound c_upper_bound c_height
+            kl vl kr vr,
+              context_iwf tl_lower_bound tr_upper_bound (h_height+1)
+                          c_lower_bound c_upper_bound c_height c
+           -> tree_iwf tl_lower_bound tl_upper_bound h_height tl
+           -> tree_iwf tr_lower_bound tr_upper_bound h_height tr
+           -> tl_upper_bound < inject kl < h_lower_bound
+           -> h_upper_bound < inject kr < tr_lower_bound
+           -> context_iwf h_lower_bound h_upper_bound h_height
+                          c_lower_bound c_upper_bound c_height
+                          (ThreeMiddleHole_c tl (kl,vl) (kr,vr) tr c)
+      | ThreeRightHoleWF :
+          forall
+            h_lower_bound h_upper_bound h_height
+            tl tl_lower_bound tl_upper_bound
+            tm tm_lower_bound tm_upper_bound
+            c c_lower_bound c_upper_bound c_height
+            kl vl kr vr,
+              context_iwf tl_lower_bound h_upper_bound (h_height+1)
+                          c_lower_bound c_upper_bound c_height c
+           -> tree_iwf tl_lower_bound tl_upper_bound h_height tl
+           -> tree_iwf tm_lower_bound tm_upper_bound h_height tm
+           -> tl_upper_bound < inject kl < tm_lower_bound
+           -> tm_upper_bound < inject kr < h_lower_bound
+           -> context_iwf h_lower_bound h_upper_bound h_height
+                          c_lower_bound c_upper_bound c_height
+                          (ThreeRightHole_c tl (kl,vl) tm (kr,vr) c).
 
-      Abort All.
-        
-  End wf.
+  Inductive location_iwf 
+      : ext_top_bot K -> ext_top_bot K -> N (* bounds and height of hole *)
+     -> ext_top_bot K -> ext_top_bot K -> N (* bounds and height when filled *)
+     -> location K V
+     -> Prop :=
+    | TwoHoleWF :
+        forall
+          t_height
+          tl tl_lower_bound tl_upper_bound
+          tr tr_lower_bound tr_upper_bound
+          c c_lower_bound c_upper_bound c_height,
+            tree_iwf tl_lower_bound tl_upper_bound t_height tl
+         -> tree_iwf tr_lower_bound tr_upper_bound t_height tr
+         -> context_iwf tl_lower_bound tr_upper_bound (t_height+1)
+                        c_lower_bound c_upper_bound c_height c
+         -> location_iwf tl_upper_bound tr_lower_bound t_height
+                         c_lower_bound c_upper_bound c_height
+                         (TwoHole_l tl tr c).
+            
+  Global Instance tree_WellFormed : WellFormed (tree K V) :=
+    { wf :=
+        fun (t:tree K V) =>
+          exists (n:N) (lb:ext_top_bot K) (ub:ext_top_bot K),
+            tree_iwf lb ub n t
+    }.
 
+  Local Ltac mysimp :=
+  match goal with
+   | [ |- tree_iwf _ _ _ (Two_t _ _ _) ] => econstructor
+   | [ |- tree_iwf _ _ _ (Three_t _ _ _ _ _) ] => econstructor
+   | [ |- context_iwf _ _ _ _ _ _ Top_c ] => econstructor
+   | [ |- context_iwf _ _ _ _ _ _ (TwoLeftHole_c _ _ _) ] => econstructor
+   | [ |- context_iwf _ _ _ _ _ _ (TwoRightHole_c _ _ _) ] => econstructor
+   | [ |- context_iwf _ _ _ _ _ _ (ThreeLeftHole_c _ _ _ _ _) ] => econstructor
+   | [ |- context_iwf _ _ _ _ _ _ (ThreeMiddleHole_c _ _ _ _ _) ] => econstructor
+   | [ |- context_iwf _ _ _ _ _ _ (ThreeRightHole_c _ _ _ _ _) ] => econstructor
+   | [ H : tree_iwf _ _ _ Null_t |- _ ] =>
+       inversion H ; subst ; clear H
+   | [ H : tree_iwf _ _ _ (Two_t _ _ _) |- _ ] =>
+       inversion H ; subst ; clear H
+   | [ H : tree_iwf _ _ _ (Three_t _ _ _ _ _) |- _ ] =>
+       inversion H ; subst ; clear H
+   | [ H : context_iwf _ _ _ _ _ _ Top_c |- _ ] =>
+       inversion H ; subst ; clear H
+   | [ H : context_iwf _ _ _ _ _ _ (TwoLeftHole_c _ _ _) |- _ ] =>
+       inversion H ; subst ; clear H
+   | [ H : context_iwf _ _ _ _ _ _ (TwoRightHole_c _ _ _) |- _ ] =>
+       inversion H ; subst ; clear H
+   | [ H : context_iwf _ _ _ _ _ _ (ThreeLeftHole_c _ _ _ _ _) |- _ ] =>
+       inversion H ; subst ; clear H
+   | [ H : context_iwf _ _ _ _ _ _ (ThreeMiddleHole_c _ _ _ _ _) |- _ ] =>
+       inversion H ; subst ; clear H
+   | [ H : context_iwf _ _ _ _ _ _ (ThreeRightHole_c _ _ _ _ _) |- _ ] =>
+       inversion H ; subst ; clear H
+   | [ H : location_iwf _ _ _ _ _ _ (TwoHole_l _ _ _) |- _ ] =>
+       inversion H ; subst ; clear H
+   | [ H : location_iwf _ _ _ _ _ _ (ThreeLeftHole_l _ _ _ _ _) |- _ ] =>
+       inversion H ; subst ; clear H
+   | [ H : location_iwf _ _ _ _ _ _ (ThreeRightHole_l _ _ _ _ _) |- _ ] =>
+       inversion H ; subst ; clear H
+   | _ => eauto
+  end.
+
+  Lemma zip_wf :
+    forall 
+      (c:context K V) (t:tree K V)
+      t_lower_bound t_upper_bound t_height
+      c_lower_bound c_upper_bound c_height,
+        tree_iwf t_lower_bound t_upper_bound t_height t
+     -> context_iwf t_lower_bound t_upper_bound t_height
+                    c_lower_bound c_upper_bound c_height c
+     -> tree_iwf c_lower_bound c_upper_bound c_height (zip t c).
+  Proof.
+    intros c.
+    induction c ; simpl ; intros ; repeat mysimp ; eapply IHc ; repeat mysimp.
+  Qed.
+  Hint Resolve zip_wf.
+
+  Lemma fuse_wf :
+    forall
+      (c1:context K V) (c2:context K V)
+      c1h_lower_bound c1h_upper_bound c1h_height
+      c1_lower_bound c1_upper_bound c1_height
+      c2_lower_bound c2_upper_bound c2_height,
+        context_iwf c1h_lower_bound c1h_upper_bound c1h_height
+                    c1_lower_bound c1_upper_bound c1_height c1
+     -> context_iwf c1_lower_bound c1_upper_bound c1_height
+                    c2_lower_bound c2_upper_bound c2_height c2
+     -> context_iwf c1h_lower_bound c1h_upper_bound c1h_height
+                    c2_lower_bound c2_upper_bound c2_height (fuse c1 c2).
+  Proof.
+    intros c1.
+    induction c1 ; simpl ; intros ; repeat mysimp.
+  Qed.
+  Hint Resolve fuse_wf.
+
+  Lemma fill_location_wf :
+    forall
+      (l:location K V) (k:K) (v:V)
+      h_lower_bound h_upper_bound h_height
+      c_lower_bound c_upper_bound c_height,
+        h_lower_bound < inject k < h_upper_bound
+     -> location_iwf h_lower_bound h_upper_bound h_height
+                     c_lower_bound c_upper_bound c_height l
+     -> tree_iwf c_lower_bound c_upper_bound c_height (fill_location (k,v) l).
+  Proof.
+    intros l.
+    induction l ; intros ; repeat mysimp.
+    eapply zip_wf ; repeat mysimp.
+  Qed.
+  Hint Resolve fill_location_wf.
+
+  Lemma locate_wf :
+    forall
+      (t:tree K V) (k:K) (c:context K V)
+      t_lower_bound t_upper_bound t_height
+      c_lower_bound c_upper_bound c_height,
+        t_lower_bound < inject k < t_upper_bound
+     -> tree_iwf t_lower_bound t_upper_bound t_height t
+     -> context_iwf t_lower_bound t_upper_bound t_height
+                    c_lower_bound c_upper_bound c_height c
+     -> exists h_lower_bound h_upper_bound,
+          h_lower_bound < inject k < h_upper_bound
+       /\ match locate k t c with
+          | inl c =>
+              context_iwf h_lower_bound h_upper_bound 0
+                          c_lower_bound c_upper_bound c_height c
+          | inr ((k,v),l) =>
+              exists h_height,
+                location_iwf h_lower_bound h_upper_bound h_height
+                             c_lower_bound c_upper_bound c_height l
+          end.
+  Proof.
+    intros t.
+    induction t ; intros ; simpl ; repeat mysimp.
+    simpl.
+    remember (k <=>! km) as cmp ; destruct cmp.
+
+    symmetry in Heqcmp.
+    eapply ord_dec_correct_eqv in Heqcmp.
+    rewrite Heqcmp in H.
+    rewrite H0 in * ; clear H0 ; clear Heqcmp.
+
+    exists tl_upper_bound.
+    exists tr_lower_bound.
+    split.
+    auto.
+    exists t_height0.
+    econstructor.
+    eapply H8.
+    eapply H9.
+    eapply H1.
+
+    assert (lt k km). admit.
+    assert (t_lower_bound < inject km < tr_lower_bound).
+      split.
+      transitivity (inject k).
+
+    eapply IHt1. 
+    eapply H.
+    eapply H8.
+
+    exists tl_upper_bound.
+
+  
 End TwoThreeTreesWF.
-
